examples/low-level/arrayAlgos.fst
@@ -1,0 +1,54 @@
+(*--build-config
+    options:--admit_fsi Set --z3timeout 10 --logQueries;
+    variables:LIB=../../lib;
+    other-files:$LIB/ext.fst $LIB/set.fsi $LIB/heap.fst $LIB/st.fst $LIB/list.fst  stack.fst listset.fst
+    st3.fst $LIB/constr.fst word.fst $LIB/seq.fsi $LIB/seq.fst array.fsi array.fst withScope.fst
+  --*)
+module ArrayAlgos
+open StructuredMem
+open MVector
+open Heap
+open Set
+open MachineWord
+open Array
+open MD5Common
+open Seq
+
+val contains : #a:Type -> smem -> array a -> GTot bool
+let contains m v = refExistsInMem (asRef v) m
+
+val sel : #a:Type -> m:smem -> v:(array a){contains m v} -> GTot (seq a)
+let sel m v = loopkupRef (asRef v) m
+
+val glength : #a:Type -> v:(array a) -> m:smem{contains m v} -> GTot nat
+let glength v m = Seq.length (sel m v)
+
+type prefixEqual  (#a:Type)
+  (v1: seq a) (v2: seq a) (p:nat{p <= length v1 /\ p<= length v2})
+  = forall (n:nat{n<p}). index v1 n = index v2 n
+
+(* Helper functions for stateful array manipulation *)
+val copy:
+  #a:Type -> s:array a -> scp :array a
+  -> WNSC unit
+     (requires (fun h -> contains h s /\ contains h scp /\ glength s h <= glength scp h))
+     (ensures (fun h0 _ h1 -> (contains h1 s) /\  (contains h1 scp)
+				      (*/\ sel h1 s = sel h1 scp *)
+              ))
+     (only (asRef scp))
+let copy s scp =
+  let ctr = salloc #nat 0 in
+  let len = Array.length s in
+  scopedWhile1
+    ctr
+    (fun ctrv -> ctrv < len)
+    (fun m -> contains m s /\ contains m scp
+        /\ len = glength s m /\ len <= glength scp m
+          /\ refExistsInMem ctr m
+          /\ (loopkupRef ctr m) <=len
+          /\ prefixEqual (sel m s) (sel m scp) (loopkupRef ctr m)
+          )
+    (only (asRef scp))
+    (fun u -> let ctrv = memread ctr in
+              (*writeIndex scp ctrv (readIndex s ctrv);*)
+              memwrite ctr (ctrv (*+1*) ))
